@prefix wurfel:  <http://fortytwo.net/2007/02/06/wurfel#> .
@prefix rdfs:    <http://www.w3.org/2000/01/rdf-schema#> .
@prefix rdf:     <http://www.w3.org/1999/02/22-rdf-syntax-ns#> .
@prefix xsd:     <http://www.w3.org/2001/XMLSchema#> .



wurfel:Apply
  rdfs:type rdfs:Class ;
  rdfs:comment "A structure representing the application of a function to an argument" .

wurfel:applyFunction
  rdfs:type rdf:Property ;
  rdfs:domain wurfel:Apply ;
  rdfs:range rdfs:Resource ;
  rdfs:comment "An applied function" .

wurfel:applyArgument
  rdfs:type rdf:Property ;
  rdfs:domain wurfel:Apply ;
  rdfs:range rdfs:Resource ;
  rdfs:comment "An applied argument" .



wurfel:PrimitiveFunction
  rdfs:type rdfs:Class ;
  rdfs:comment "A built-in function" .

wurfel:returnType
  rdfs:type rdf:Property ;
  rdfs:domain wurfel:PrimitiveFunction ;
  rdfs:range rdfs:DataType ;
  rdfs:comment "The data type of the return value of a function" .

wurfel:parameters
  rdfs:type rdf:Property ;
  rdfs:domain wurfel:PrimitiveFunction ;
  rdfs:range wurfel:ParameterList ;
  rdfs:comment "" .

wurfel:Parameter
  rdfs:type rdfs:Class ;
  rdfs:comment "A formal argument to a function" .

# Note: I don't know how to make this a list of wurfel:Parameter's specifically.
wurfel:ParameterList
  rdfs:type rdfs:Class ;
  rdfs:subClassOf rdf:List .

wurfel:parameterType
  rdfs:type rdf:Property ;
  rdfs:domain wurfel:Parameter ;
  rdfs:range xsd:string ;
  rdfs:comment "A helpful name for the parameter." .

wurfel:parameterType
  rdfs:type rdf:Property ;
  rdfs:domain wurfel:Parameter ;
  rdfs:range rdfs:DataType ;
  rdfs:comment "The data type of a formal argument to a function" .

wurfel:parameterTransparency
  rdfs:type rdf:Property ;
  rdfs:domain wurfel:Parameter ;
  rdfs:range xsd:boolean ;
  rdfs:comment "A condition indicating whether the application of a function may have side-effects on a particular argument" .



wurfel:Combinator
  rdfs:type rdfs:Class ;
  rdfs:comment "A function with no free variables" .

wurfel:combinatorArity
  rdfs:type rdf:Property ;
  rdfs:domain wurfel:Combinator ;
  rdfs:range xsd:integer ;
  rdfs:comment "The number of formal arguments consumed by a combinator" .



# Note: for now, these container functions are considered combinators, as they
#       are applied on the same level as combinators.  Renaming them, along with
#       the combinators, to something like "MetaFunction" might be a good idea.
wurfel:and
  rdfs:type wurfel:Combinator ;
  wurfel:combinatorArity 2 ;
  rdfs:comment "Finds the intersection of one set with another set" .

wurfel:or
  rdfs:type wurfel:Combinator ;
  wurfel:combinatorArity 2 ;
  rdfs:comment "Finds the union of one set with another set" .

wurfel:without
  rdfs:type wurfel:Combinator ;
  wurfel:combinatorArity 2 ;
  rdfs:comment "Finds the intersection of one set with the complement of another set" .
