@prefix cache: <http://fortytwo.net/2007/07/ripple/cache#>.
@prefix rdf:   <http://www.w3.org/1999/02/22-rdf-syntax-ns#> .
@prefix rdfs:  <http://www.w3.org/2000/01/rdf-schema#> .

cache:Cache
	a rdfs:Class;
	rdfs:comment "a resource representing a Ripple web cache";
	.

cache:InformationResource
	a rdfs:Class;
	.

cache:includes
	a rdf:Property;
	rdfs:domain cache:Cache;
	rdfs:range cache:InformationResource;
	rdfs:comment "indicates that a document has been successfully dereferenced";
	.

cache:excludes
	a rdf:Property;
	rdfs:domain cache:Cache;
	rdfs:range cache:InformationResource;
	rdfs:comment "indicates that a document has been tried but not successfully dereferenced";
	.

cache:lastAccessed
	a rdf:Property;
	rdfs:domain cache:InformationResource;
	rdfs:range xsd:dateTime;
	rdfs:comment "the most recent date and time at which a document was requested"
	.

<urn:net.fortytwo.ripple.store.meta>
	a cache:Cache;
	rdfs:comment "an indexical resource which stands for 'this cache'";
	.
